Prove reorder rel-fence and refactor

src/opt/itree/iReorderAbort.v
@@ -39,7 +39,8 @@ Inductive reorder_abort: forall R (i2:MemE.t R), Prop :=
     reorder_abort (MemE.read l2 o2)
 | reorder_abort_store
     l2 v2 o2
-    (ORD: Ordering.le o2 Ordering.acqrel):
+    (ORD21: Ordering.le o2 Ordering.acqrel)
+    (ORD22: Ordering.le Ordering.plain o2):
     reorder_abort (MemE.write l2 v2 o2)
 | reorder_abort_fence
     or2 ow2
@@ -48,66 +49,24 @@ Inductive reorder_abort: forall R (i2:MemE.t R), Prop :=
     reorder_abort (MemE.fence or2 ow2)
 .
 
-Inductive sim_abort: forall R
-                            (st_src:itree MemE.t (void * R)%type) (lc_src:Local.t) (sc1_src:TimeMap.t) (mem1_src:Memory.t)
-                            (st_tgt:itree MemE.t (void * R)%type) (lc_tgt:Local.t) (sc1_tgt:TimeMap.t) (mem1_tgt:Memory.t), Prop :=
+Inductive sim_abort:
+  forall R (st_src:itree MemE.t (void * R)%type) (lc_src:Local.t) (sc1_src:TimeMap.t) (mem1_src:Memory.t), Prop :=
 | sim_abort_intro
     R (i2: MemE.t R)
     lc1_src sc1_src mem1_src
-    lc1_tgt sc1_tgt mem1_tgt
     (REORDER: reorder_abort i2)
     (FAILURE: Local.failure_step lc1_src)
-    (LOCAL: sim_local SimPromises.bot lc1_src lc1_tgt)
-    (SC: TimeMap.le sc1_src sc1_tgt)
-    (MEMORY: sim_memory mem1_src mem1_tgt)
     (WF_SRC: Local.wf lc1_src mem1_src)
-    (WF_TGT: Local.wf lc1_tgt mem1_tgt)
     (SC_SRC: Memory.closed_timemap sc1_src mem1_src)
-    (SC_TGT: Memory.closed_timemap sc1_tgt mem1_tgt)
-    (MEM_SRC: Memory.closed mem1_src)
-    (MEM_TGT: Memory.closed mem1_tgt)
-    k
-  :
+    (MEM_SRC: Memory.closed mem1_src):
     @sim_abort
-      R
-      (Vis i2 (fun v2 => Vis (MemE.abort) (fun v1 => Ret (v1, v2)))) lc1_src sc1_src mem1_src
-      (Vis MemE.abort k) lc1_tgt sc1_tgt mem1_tgt
+      R (Vis i2 (fun v2 => Vis (MemE.abort) (fun v1 => Ret (v1, v2)))) lc1_src sc1_src mem1_src
 .
-
-Lemma sim_abort_mon
-      R
-      st_src lc_src sc1_src mem1_src
-      st_tgt lc_tgt sc1_tgt mem1_tgt
-      sc2_src mem2_src
-      sc2_tgt mem2_tgt
-      (SIM1: sim_abort st_src lc_src sc1_src mem1_src
-                       st_tgt lc_tgt sc1_tgt mem1_tgt)
-      (SC_FUTURE_SRC: TimeMap.le sc1_src sc2_src)
-      (SC_FUTURE_TGT: TimeMap.le sc1_tgt sc2_tgt)
-      (MEM_FUTURE_SRC: Memory.future_weak mem1_src mem2_src)
-      (MEM_FUTURE_TGT: Memory.future_weak mem1_tgt mem2_tgt)
-      (SC1: TimeMap.le sc2_src sc2_tgt)
-      (MEM1: sim_memory mem2_src mem2_tgt)
-      (WF_SRC: Local.wf lc_src mem2_src)
-      (WF_TGT: Local.wf lc_tgt mem2_tgt)
-      (SC_SRC: Memory.closed_timemap sc2_src mem2_src)
-      (SC_TGT: Memory.closed_timemap sc2_tgt mem2_tgt)
-      (MEM_SRC: Memory.closed mem2_src)
-      (MEM_TGT: Memory.closed mem2_tgt):
-  @sim_abort R
-             st_src lc_src sc2_src mem2_src
-             st_tgt lc_tgt sc2_tgt mem2_tgt.
-Proof.
-  dependent destruction SIM1. econs; eauto.
-Qed.
 
 Lemma sim_abort_steps_failure
       R
       st1_src lc1_src sc1_src mem1_src
-      st1_tgt lc1_tgt sc1_tgt mem1_tgt
-      (SIM: @sim_abort R
-                       st1_src lc1_src sc1_src mem1_src
-                       st1_tgt lc1_tgt sc1_tgt mem1_tgt):
+      (SIM: @sim_abort R st1_src lc1_src sc1_src mem1_src):
   Thread.steps_failure (Thread.mk (lang (void * R)%type) st1_src lc1_src sc1_src mem1_src).
 Proof.
   destruct SIM. inv FAILURE. unfold Thread.steps_failure.
@@ -119,14 +78,17 @@ Proof.
     + econs 2; try refl. econs.
       * econs. econs 2. econs; [|econs 2]; eauto. econs. econs.
       * ss.
-    + econs 2. econs.
+    + econs 2. econs; [|econs 7].
       * econs; eauto.
-      * econs. econs. ii.
+      * econs. ii.
         rewrite <- TVIEW. rewrite <- PROMISES in *. eauto.
+    + ss.
   - (* store *)
     exploit (@LowerPromises.steps_promises_rel
-               (lang (void * unit)%type) (Thread.mk (lang (void * unit)%type) (Vis (MemE.write l2 v2 o2) (fun v2 => Vis (MemE.abort) (fun v1 => Ret (v1, v2))))
-                                                    lc1_src sc1_src mem1_src)); s; eauto.
+               (lang (void * unit)%type)
+               (Thread.mk (lang (void * unit)%type)
+                          (Vis (MemE.write l2 v2 o2) (fun v2 => Vis (MemE.abort) (fun v1 => Ret (v1, v2))))
+                          lc1_src sc1_src mem1_src)); s; eauto.
     i. des. destruct e2. ss.
     exploit LowerPromises.rtc_opt_promise_step_future; eauto. s. i. des. subst.
     hexploit LowerPromises.promises_rel_promise_consistent; eauto. i.
@@ -137,11 +99,16 @@ Proof.
     + eapply rtc_n1; eauto. econs.
       * econs. econs 2. econs; [|econs 3; eauto]. econs. econs.
       * ss.
-    + econs 2. econs; [econs; econs|]. econs. econs. ss.
+    + econs 2. econs; [|econs 7].
+      * econs.
+      * econs. ss.
+    + ss.
   - (* fence *)
     exploit (@LowerPromises.steps_promises_rel
-               (lang (void * unit)%type) (Thread.mk (lang (void * unit)%type) (Vis (MemE.fence or2 ow2) (fun v2 => Vis (MemE.abort) (fun v1 => Ret (v1, v2))))
-                                      lc1_src sc1_src mem1_src)); s; eauto.
+               (lang (void * unit)%type)
+               (Thread.mk (lang (void * unit)%type)
+                          (Vis (MemE.fence or2 ow2) (fun v2 => Vis (MemE.abort) (fun v1 => Ret (v1, v2))))
+                          lc1_src sc1_src mem1_src)); s; eauto.
     i. des. destruct e2. ss.
     exploit LowerPromises.rtc_opt_promise_step_future; eauto. s. i. des. inv STATE.
     hexploit LowerPromises.promises_rel_promise_consistent; eauto. i.
@@ -153,8 +120,9 @@ Proof.
     + eapply rtc_n1; eauto. econs.
       * econs. econs 2. econs; [|econs 5; eauto]. econs. econs.
       * ss.
-    + econs 2. econs; [econs; econs|]. econs. econs.
-      exploit fence_step_future; eauto. i. des.
-      ii. rewrite <- PROMISES in *. rewrite <- TVIEW0. eauto.
-  Unshelve. all: try exact ITree.spin.
+    + econs 2. econs; [|econs 7].
+      * econs.
+      * econs. exploit fence_step_future; eauto. i. des.
+        ii. rewrite <- PROMISES in *. rewrite <- TVIEW0. eauto.
+    + ss.
 Qed.
