src/opt/while/ReorderAbort.v
@@ -49,58 +49,22 @@ Inductive reorder_abort: forall (i2:Instr.t), Prop :=
     reorder_abort (Instr.fence or2 ow2)
 .
 
-Inductive sim_abort: forall (st_src:(Language.state lang)) (lc_src:Local.t) (sc1_src:TimeMap.t) (mem1_src:Memory.t)
-                       (st_tgt:(Language.state lang)) (lc_tgt:Local.t) (sc1_tgt:TimeMap.t) (mem1_tgt:Memory.t), Prop :=
+Inductive sim_abort: forall (st_src:(Language.state lang)) (lc_src:Local.t) (sc1_src:TimeMap.t) (mem1_src:Memory.t), Prop :=
 | sim_abort_intro
     rs i2
     lc1_src sc1_src mem1_src
-    lc1_tgt sc1_tgt mem1_tgt
     (REORDER: reorder_abort i2)
     (FAILURE: Local.failure_step lc1_src)
-    (LOCAL: sim_local SimPromises.bot lc1_src lc1_tgt)
-    (SC: TimeMap.le sc1_src sc1_tgt)
-    (MEMORY: sim_memory mem1_src mem1_tgt)
     (WF_SRC: Local.wf lc1_src mem1_src)
-    (WF_TGT: Local.wf lc1_tgt mem1_tgt)
     (SC_SRC: Memory.closed_timemap sc1_src mem1_src)
-    (SC_TGT: Memory.closed_timemap sc1_tgt mem1_tgt)
-    (MEM_SRC: Memory.closed mem1_src)
-    (MEM_TGT: Memory.closed mem1_tgt):
+    (MEM_SRC: Memory.closed mem1_src):
     sim_abort
       (State.mk rs [Stmt.instr i2; Stmt.instr Instr.abort]) lc1_src sc1_src mem1_src
-      (State.mk rs [Stmt.instr i2]) lc1_tgt sc1_tgt mem1_tgt
 .
-
-Lemma sim_abort_mon
-      st_src lc_src sc1_src mem1_src
-      st_tgt lc_tgt sc1_tgt mem1_tgt
-      sc2_src mem2_src
-      sc2_tgt mem2_tgt
-      (SIM1: sim_abort st_src lc_src sc1_src mem1_src
-                       st_tgt lc_tgt sc1_tgt mem1_tgt)
-      (SC_FUTURE_SRC: TimeMap.le sc1_src sc2_src)
-      (SC_FUTURE_TGT: TimeMap.le sc1_tgt sc2_tgt)
-      (MEM_FUTURE_SRC: Memory.future_weak mem1_src mem2_src)
-      (MEM_FUTURE_TGT: Memory.future_weak mem1_tgt mem2_tgt)
-      (SC1: TimeMap.le sc2_src sc2_tgt)
-      (MEM1: sim_memory mem2_src mem2_tgt)
-      (WF_SRC: Local.wf lc_src mem2_src)
-      (WF_TGT: Local.wf lc_tgt mem2_tgt)
-      (SC_SRC: Memory.closed_timemap sc2_src mem2_src)
-      (SC_TGT: Memory.closed_timemap sc2_tgt mem2_tgt)
-      (MEM_SRC: Memory.closed mem2_src)
-      (MEM_TGT: Memory.closed mem2_tgt):
-  sim_abort st_src lc_src sc2_src mem2_src
-            st_tgt lc_tgt sc2_tgt mem2_tgt.
-Proof.
-  inv SIM1. econs; eauto.
-Qed.
 
 Lemma sim_abort_steps_failure
       st1_src lc1_src sc1_src mem1_src
-      st1_tgt lc1_tgt sc1_tgt mem1_tgt
-      (SIM: sim_abort st1_src lc1_src sc1_src mem1_src
-                      st1_tgt lc1_tgt sc1_tgt mem1_tgt):
+      (SIM: sim_abort st1_src lc1_src sc1_src mem1_src):
   Thread.steps_failure (Thread.mk lang st1_src lc1_src sc1_src mem1_src).
 Proof.
   inv SIM. inv FAILURE. unfold Thread.steps_failure.
