src/opt/while/ReorderStore.v
@@ -63,7 +63,7 @@ Inductive reorder_store l1 v1 o1: forall (i2:Instr.t), Prop :=
 
 Inductive sim_store: forall (st_src:(Language.state lang)) (lc_src:Local.t) (sc1_src:TimeMap.t) (mem1_src:Memory.t)
                        (st_tgt:(Language.state lang)) (lc_tgt:Local.t) (sc1_tgt:TimeMap.t) (mem1_tgt:Memory.t), Prop :=
-| sim_store_write
+| sim_store_intro
     l1 f1 t1 v1 released1 o1 i2 rs
     lc1_src sc1_src mem1_src
     lc1_tgt sc1_tgt mem1_tgt
@@ -72,24 +72,6 @@ Inductive sim_store: forall (st_src:(Language.state lang)) (lc_src:Local.t) (sc1
     (FULFILL: fulfill_step lc1_src sc1_src l1 f1 t1 (RegFile.eval_value rs v1) None released1 o1 lc2_src sc2_src)
     (LOCAL: sim_local SimPromises.bot lc2_src lc1_tgt)
     (SC: TimeMap.le sc2_src sc1_tgt)
-    (MEMORY: sim_memory mem1_src mem1_tgt)
-    (WF_SRC: Local.wf lc1_src mem1_src)
-    (WF_TGT: Local.wf lc1_tgt mem1_tgt)
-    (SC_SRC: Memory.closed_timemap sc1_src mem1_src)
-    (SC_TGT: Memory.closed_timemap sc1_tgt mem1_tgt)
-    (MEM_SRC: Memory.closed mem1_src)
-    (MEM_TGT: Memory.closed mem1_tgt):
-    sim_store
-      (State.mk rs [Stmt.instr i2; Stmt.instr (Instr.store l1 v1 o1)]) lc1_src sc1_src mem1_src
-      (State.mk rs [Stmt.instr i2]) lc1_tgt sc1_tgt mem1_tgt
-| sim_store_racy_write
-    l1 v1 o1 i2 rs
-    lc1_src sc1_src mem1_src
-    lc1_tgt sc1_tgt mem1_tgt
-    (REORDER: reorder_store l1 v1 o1 i2)
-    (RACY_WRITE: Local.racy_write_step lc1_src mem1_src l1 o1)
-    (LOCAL: sim_local SimPromises.bot lc1_src lc1_tgt)
-    (SC: TimeMap.le sc1_src sc1_tgt)
     (MEMORY: sim_memory mem1_src mem1_tgt)
     (WF_SRC: Local.wf lc1_src mem1_src)
     (WF_TGT: Local.wf lc1_tgt mem1_tgt)
@@ -125,10 +107,8 @@ Lemma sim_store_mon
             st_tgt lc_tgt sc2_tgt mem2_tgt.
 Proof.
   inv SIM1.
-  - exploit future_fulfill_step; try exact FULFILL; eauto; try refl.
-    i. des. econs; eauto.
-  - exploit future_racy_write_step; try exact RACY_WRITE; eauto.
-    i. des. econs 2; eauto.
+  exploit future_fulfill_step; try exact FULFILL; eauto; try refl.
+  i. des. econs; eauto.
 Qed.
 
 Lemma sim_store_step
@@ -140,144 +120,97 @@ Lemma sim_store_step
                      st1_src lc1_src sc1_src mem1_src
                      st1_tgt lc1_tgt sc1_tgt mem1_tgt.
 Proof.
-  inv SIM.
-  { (* write *)
-    ii.
-    exploit fulfill_step_future; eauto; try viewtac. i. des.
-    inv STEP_TGT; [inv STEP|inv STEP; inv LOCAL0];
-      try (inv STATE; inv INSTR; inv REORDER); ss.
-    - (* promise *)
-      right.
-      exploit Local.promise_step_future; eauto. i. des.
-      exploit sim_local_promise; try exact LOCAL0; (try by etrans; eauto); eauto. i. des.
-      exploit reorder_fulfill_promise; try exact FULFILL; try exact STEP_SRC; eauto. i. des.
-      exploit Local.promise_step_future; eauto. i. des.
-      esplits.
-      + ss.
-      + eauto.
-      + econs 2. econs 1. econs; eauto.
-      + auto.
-      + etrans; eauto.
-      + auto.
-      + right. econs; eauto.
-        eapply Memory.future_closed_timemap; eauto.
-    - (* load *)
-      right.
-      exploit sim_local_read; try exact LOCAL0; (try by etrans; eauto); eauto; try refl. i. des.
-      exploit reorder_fulfill_read; try exact FULFILL; try exact STEP_SRC; eauto. i. des.
-      exploit Local.read_step_future; try exact STEP1; eauto. i. des.
-      exploit fulfill_write_sim_memory; eauto; try by viewtac. i. des.
-      esplits.
-      + ss.
-      + econs 2; eauto. econs.
-        * econs. econs 2. econs; [|econs 2]; eauto. econs. econs.
-        * auto.
-      + econs 2. econs 2. econs; [|econs 3]; eauto. econs.
-        erewrite <- RegFile.eq_except_value; eauto.
-        * econs.
-        * symmetry. eauto.
-        * apply RegFile.eq_except_singleton.
-      + auto.
-      + auto.
-      + etrans; eauto.
-      + left. eapply paco11_mon; [apply sim_stmts_nil|]; ss.
-    - (* store *)
-      right.
-      hexploit sim_local_write_bot; try exact LOCAL1;
-        try match goal with
-            | [|- is_true (Ordering.le _ _)] => refl
-            end; eauto; try refl; try by viewtac. i. des.
-      hexploit reorder_fulfill_write_sim_memory; try exact FULFILL; try exact STEP_SRC; eauto; try by viewtac. i. des.
-      exploit Local.write_step_future; try exact STEP1; eauto; try by viewtac. i. des.
-      exploit fulfill_write_sim_memory; eauto; try by viewtac. i. des.
-      esplits.
-      + ss.
-      + econs 2; eauto. econs.
-        * econs. econs 2. econs; [|econs 3]; eauto. econs. econs.
-        * auto.
-      + econs 2. econs 2. econs; [|econs 3]; eauto. econs. econs.
-      + auto.
-      + etrans; eauto.
-      + etrans; eauto. etrans; eauto.
-      + left. eapply paco11_mon; [apply sim_stmts_nil|]; ss.
-        etrans; eauto.
-    - (* na write *)
-      inv LOCAL1. destruct ord; ss.
-    - (* racy read *)
-      right.
-      exploit sim_local_racy_read; try exact LOCAL1; eauto; try refl. i. des.
-      exploit reorder_fulfill_racy_read; try exact FULFILL; eauto. i. des.
-      exploit fulfill_write_sim_memory; eauto. i. des.
-      esplits.
-      + ss.
-      + econs 2; eauto. econs.
-        * econs. econs 2. econs; [|econs 9]; eauto. econs. econs.
-        * auto.
-      + econs 2. econs 2. econs; [|econs 3]; eauto. econs.
-        erewrite <- RegFile.eq_except_value; eauto.
-        * econs.
-        * symmetry. eauto.
-        * apply RegFile.eq_except_singleton.
-      + auto.
-      + ss.
-      + etrans; eauto.
-      + left. eapply paco11_mon; [apply sim_stmts_nil|]; ss.
-    - (* racy write *)
-      left.
-      exploit sim_local_racy_write; try exact LOCAL1;
-        try match goal with
-            | [|- is_true (Ordering.le _ _)] => refl
-            end; eauto; try refl. i. des.
-      exploit reorder_fulfill_racy_write; try exact FULFILL; eauto. i. des.
-      unfold Thread.steps_failure.
-      esplits; try refl.
-      + econs 2. econs; [|econs 10]; eauto. econs. econs.
-      + ss.
-  }
-
-  { (* racy write *)
-    ii. left. unfold Thread.steps_failure.
-    inv REORDER.
-    - (* load *)
-      exploit progress_read_step_cur; try exact WF_SRC; eauto. i. des.
-      exploit read_step_cur_future; try exact READ; eauto. i. des.
-      esplits.
-      + econs 2; try refl. econs.
-        * econs. econs 2. econs; [|econs 2]; eauto. econs. econs.
-        * ss.
-      + econs 2. econs; [|econs 10].
-        * econs. econs.
-        * inv RACY_WRITE. econs; eauto; try congr.
-          { inv RACE. econs. congr. }
-          { ii. rewrite <- PROMISES, <- TVIEW in *. eauto. }
-      + ss.
-    - (* store *)
-      exploit (@LowerPromises.steps_promises_rel
-                 lang (Thread.mk lang (State.mk rs [Stmt.instr (Instr.store l2 v2 o2); Stmt.instr (Instr.store l1 v1 o1)])
-                                 lc1_src sc1_src mem1_src)); s; eauto.
-      i. des. destruct e2, state. ss.
-      exploit LowerPromises.rtc_opt_promise_step_future; eauto. s. i. des. inv STATE.
-      hexploit LowerPromises.promises_rel_promise_consistent; try apply RACY_WRITE; eauto. i.
-      hexploit LowerPromises.promises_rel_nonsynch; eauto. i.
-      exploit Thread.rtc_tau_step_future; try exact STEPS0; eauto. s. i. des.
-      exploit write_step_consistent; try exact WF2; eauto. i. des.
-      esplits.
-      + eapply rtc_n1; eauto. econs.
-        * econs. econs 2. econs; [|econs 3; eauto]. econs. econs.
-        * ss.
-      + econs 2. econs; [|econs 10].
-        * econs. econs.
-        * inv RACY_WRITE.
-          exploit Thread.rtc_tau_step_non_promised; try exact STEPS0; eauto. s. i. des.
-          exploit Local.program_step_non_promised; [econs 3|..]; try exact STEP; eauto. i. des.
-          econs; eauto; try congr.
-          inv RACE. econs. rewrite TVIEW in TS.
-          inv STEP. ss.
-          apply TimeFacts.join_spec_lt; auto.
-          unfold TimeMap.singleton, Loc.LocFun.add, Loc.LocFun.init, Loc.LocFun.find. condtac; ss.
-          eapply TimeFacts.le_lt_lt; eauto. apply Time.bot_spec.
-      + ss.
-  }
+  inv SIM. ii.
+  exploit fulfill_step_future; eauto; try viewtac. i. des.
+  inv STEP_TGT; [inv STEP|inv STEP; inv LOCAL0];
+    try (inv STATE; inv INSTR; inv REORDER); ss.
+  - (* promise *)
+    right.
+    exploit Local.promise_step_future; eauto. i. des.
+    exploit sim_local_promise; try exact LOCAL0; (try by etrans; eauto); eauto. i. des.
+    exploit reorder_fulfill_promise; try exact FULFILL; try exact STEP_SRC; eauto. i. des.
+    exploit Local.promise_step_future; eauto. i. des.
+    esplits.
+    + ss.
+    + eauto.
+    + econs 2. econs 1. econs; eauto.
+    + auto.
+    + etrans; eauto.
+    + auto.
+    + right. econs; eauto.
+      eapply Memory.future_closed_timemap; eauto.
+  - (* load *)
+    right.
+    exploit sim_local_read; try exact LOCAL0; (try by etrans; eauto); eauto; try refl. i. des.
+    exploit reorder_fulfill_read; try exact FULFILL; try exact STEP_SRC; eauto. i. des.
+    exploit Local.read_step_future; try exact STEP1; eauto. i. des.
+    exploit fulfill_write_sim_memory; eauto; try by viewtac. i. des.
+    esplits.
+    + ss.
+    + econs 2; eauto. econs.
+      * econs. econs 2. econs; [|econs 2]; eauto. econs. econs.
+      * auto.
+    + econs 2. econs 2. econs; [|econs 3]; eauto. econs.
+      erewrite <- RegFile.eq_except_value; eauto.
+      * econs.
+      * symmetry. eauto.
+      * apply RegFile.eq_except_singleton.
+    + auto.
+    + auto.
+    + etrans; eauto.
+    + left. eapply paco11_mon; [apply sim_stmts_nil|]; ss.
+  - (* store *)
+    right.
+    hexploit sim_local_write_bot; try exact LOCAL1;
+      try match goal with
+          | [|- is_true (Ordering.le _ _)] => refl
+          end; eauto; try refl; try by viewtac. i. des.
+    hexploit reorder_fulfill_write_sim_memory; try exact FULFILL; try exact STEP_SRC; eauto; try by viewtac. i. des.
+    exploit Local.write_step_future; try exact STEP1; eauto; try by viewtac. i. des.
+    exploit fulfill_write_sim_memory; eauto; try by viewtac. i. des.
+    esplits.
+    + ss.
+    + econs 2; eauto. econs.
+      * econs. econs 2. econs; [|econs 3]; eauto. econs. econs.
+      * auto.
+    + econs 2. econs 2. econs; [|econs 3]; eauto. econs. econs.
+    + auto.
+    + etrans; eauto.
+    + etrans; eauto. etrans; eauto.
+    + left. eapply paco11_mon; [apply sim_stmts_nil|]; ss.
+      etrans; eauto.
+  - (* na write *)
+    inv LOCAL1. destruct ord; ss.
+  - (* racy read *)
+    right.
+    exploit sim_local_racy_read; try exact LOCAL1; eauto; try refl. i. des.
+    exploit reorder_fulfill_racy_read; try exact FULFILL; eauto. i. des.
+    exploit fulfill_write_sim_memory; eauto. i. des.
+    esplits.
+    + ss.
+    + econs 2; eauto. econs.
+      * econs. econs 2. econs; [|econs 9]; eauto. econs. econs.
+      * auto.
+    + econs 2. econs 2. econs; [|econs 3]; eauto. econs.
+      erewrite <- RegFile.eq_except_value; eauto.
+      * econs.
+      * symmetry. eauto.
+      * apply RegFile.eq_except_singleton.
+    + auto.
+    + ss.
+    + etrans; eauto.
+    + left. eapply paco11_mon; [apply sim_stmts_nil|]; ss.
+  - (* racy write *)
+    left.
+    exploit sim_local_racy_write; try exact LOCAL1;
+      try match goal with
+          | [|- is_true (Ordering.le _ _)] => refl
+          end; eauto; try refl. i. des.
+    exploit reorder_fulfill_racy_write; try exact FULFILL; eauto. i. des.
+    unfold Thread.steps_failure.
+    esplits; try refl.
+    + econs 2. econs; [|econs 10]; eauto. econs. econs.
+    + ss.
 Qed.
 
 Lemma sim_store_sim_thread:
@@ -287,75 +220,103 @@ Proof.
   - inv TERMINAL_TGT. inv PR; ss.
   - exploit sim_store_mon; eauto. i.
     inversion x0.
-    { subst.
-      exploit (progress_program_step_non_update rs i2 nil); eauto.
-      { inv x0; inv REORDER0; ss. }
-      i. des.
-      destruct th2. exploit sim_store_step; eauto.
-      { econs 2. eauto. }
-      i. des; eauto.
-      + exploit Thread.program_step_promises_bot; eauto. s. i.
-        exploit Thread.rtc_tau_step_future; eauto. s. i. des.
-        exploit Thread.opt_step_future; eauto. s. i. des.
-        exploit Thread.program_step_future; eauto. s. i. des.
-        punfold SIM. exploit SIM; try apply SC3; eauto; try refl.
-        { exploit Thread.program_step_promises_bot; eauto. s. i.
-          eapply Local.bot_promise_consistent; eauto. }
-        s. i. des.
-        exploit PROMISES; eauto. i. des.
-        * left.
-          unfold Thread.steps_failure in *. des.
-          esplits; [|eauto|]; ss.
-          etrans; eauto. etrans; [|eauto].
-          inv STEP_SRC; eauto. econs 2; eauto. econs; eauto.
-          { econs. eauto. }
-          { etrans; eauto.
-            destruct e; by inv STEP; inv STATE; inv INSTR; inv REORDER. }
-        * right.
-          esplits; [|eauto].
-          etrans; eauto. etrans; [|eauto].
-          inv STEP_SRC; eauto. econs 2; eauto. econs; eauto.
-          { econs. eauto. }
-          { etrans; eauto.
-            destruct e; by inv STEP; inv STATE; inv INSTR; inv REORDER. }
-      + inv SIM; inv STEP; inv STATE.
-    }
-    { subst.
-      exploit (progress_program_step_non_update rs i2 nil); eauto.
-      { inv x0; inv REORDER0; ss. }
-      i. des.
-      destruct th2. exploit sim_store_step; eauto.
-      { econs 2. eauto. }
-      i. des; eauto.
-      + exploit Thread.program_step_promises_bot; eauto. s. i.
-        exploit Thread.rtc_tau_step_future; eauto. s. i. des.
-        exploit Thread.opt_step_future; eauto. s. i. des.
-        exploit Thread.program_step_future; eauto. s. i. des.
-        punfold SIM. exploit SIM; try apply SC3; eauto; try refl.
-        { exploit Thread.program_step_promises_bot; eauto. s. i.
-          eapply Local.bot_promise_consistent; eauto. }
-        s. i. des.
-        exploit PROMISES; eauto. i. des.
-        * left.
-          unfold Thread.steps_failure in *. des.
-          esplits; [|eauto|]; ss.
-          etrans; eauto. etrans; [|eauto].
-          inv STEP_SRC; eauto. econs 2; eauto. econs; eauto.
-          { econs. eauto. }
-          { etrans; eauto.
-            destruct e; by inv STEP; inv STATE; inv INSTR; inv REORDER. }
-        * right.
-          esplits; [|eauto].
-          etrans; eauto. etrans; [|eauto].
-          inv STEP_SRC; eauto. econs 2; eauto. econs; eauto.
-          { econs. eauto. }
-          { etrans; eauto.
-            destruct e; by inv STEP; inv STATE; inv INSTR; inv REORDER. }
-      + inv SIM; inv STEP; inv STATE.
-    }
+    subst.
+    exploit (progress_program_step_non_update rs i2 nil); eauto.
+    { inv x0; inv REORDER0; ss. }
+    i. des.
+    destruct th2. exploit sim_store_step; eauto.
+    { econs 2. eauto. }
+    i. des; eauto.
+    + exploit Thread.program_step_promises_bot; eauto. s. i.
+      exploit Thread.rtc_tau_step_future; eauto. s. i. des.
+      exploit Thread.opt_step_future; eauto. s. i. des.
+      exploit Thread.program_step_future; eauto. s. i. des.
+      punfold SIM. exploit SIM; try apply SC3; eauto; try refl.
+      { exploit Thread.program_step_promises_bot; eauto. s. i.
+        eapply Local.bot_promise_consistent; eauto. }
+      s. i. des.
+      exploit PROMISES; eauto. i. des.
+      * left.
+        unfold Thread.steps_failure in *. des.
+        esplits; [|eauto|]; ss.
+        etrans; eauto. etrans; [|eauto].
+        inv STEP_SRC; eauto. econs 2; eauto. econs; eauto.
+        { econs. eauto. }
+        { etrans; eauto.
+          destruct e; by inv STEP; inv STATE; inv INSTR; inv REORDER. }
+      * right.
+        esplits; [|eauto].
+        etrans; eauto. etrans; [|eauto].
+        inv STEP_SRC; eauto. econs 2; eauto. econs; eauto.
+        { econs. eauto. }
+        { etrans; eauto.
+          destruct e; by inv STEP; inv STATE; inv INSTR; inv REORDER. }
+    + inv SIM; inv STEP; inv STATE.
   - exploit sim_store_mon; eauto. i. des.
     exploit sim_store_step; eauto. i. des; eauto.
     + right. esplits; eauto.
       left. eapply paco11_mon; eauto. ss.
     + right. esplits; eauto.
+Qed.
+
+Inductive sim_store_race:
+  forall (st_src:(Language.state lang)) (lc_src:Local.t) (sc1_src:TimeMap.t) (mem1_src:Memory.t), Prop :=
+| sim_store_race_intro
+    l1 v1 o1 i2 rs
+    lc1_src sc1_src mem1_src
+    (REORDER: reorder_store l1 v1 o1 i2)
+    (RACY_WRITE: Local.racy_write_step lc1_src mem1_src l1 o1)
+    (WF_SRC: Local.wf lc1_src mem1_src)
+    (SC_SRC: Memory.closed_timemap sc1_src mem1_src)
+    (MEM_SRC: Memory.closed mem1_src):
+    sim_store_race
+      (State.mk rs [Stmt.instr i2; Stmt.instr (Instr.store l1 v1 o1)]) lc1_src sc1_src mem1_src
+.
+
+Lemma sim_store_race_steps_failure
+      st1_src lc1_src sc1_src mem1_src
+      (SIM: sim_store_race st1_src lc1_src sc1_src mem1_src):
+  Thread.steps_failure (Thread.mk lang st1_src lc1_src sc1_src mem1_src).
+Proof.
+  unfold Thread.steps_failure.
+  inv SIM. inv REORDER.
+  - (* load *)
+    exploit progress_read_step_cur; try exact WF_SRC; eauto. i. des.
+    exploit read_step_cur_future; try exact READ; eauto. i. des.
+    esplits.
+    + econs 2; try refl. econs.
+      * econs. econs 2. econs; [|econs 2]; eauto. econs. econs.
+      * ss.
+    + econs 2. econs; [|econs 10].
+      * econs. econs.
+      * inv RACY_WRITE. econs; eauto; try congr.
+        { inv RACE. econs. congr. }
+        { ii. rewrite <- PROMISES, <- TVIEW in *. eauto. }
+    + ss.
+  - (* store *)
+    exploit (@LowerPromises.steps_promises_rel
+               lang (Thread.mk lang (State.mk rs [Stmt.instr (Instr.store l2 v2 o2); Stmt.instr (Instr.store l1 v1 o1)])
+                               lc1_src sc1_src mem1_src)); s; eauto.
+    i. des. destruct e2, state. ss.
+    exploit LowerPromises.rtc_opt_promise_step_future; eauto. s. i. des. inv STATE.
+    hexploit LowerPromises.promises_rel_promise_consistent; try apply RACY_WRITE; eauto. i.
+    hexploit LowerPromises.promises_rel_nonsynch; eauto. i.
+    exploit Thread.rtc_tau_step_future; try exact STEPS0; eauto. s. i. des.
+    exploit write_step_consistent; try exact WF2; eauto. i. des.
+    esplits.
+    + eapply rtc_n1; eauto. econs.
+      * econs. econs 2. econs; [|econs 3; eauto]. econs. econs.
+      * ss.
+    + econs 2. econs; [|econs 10].
+      * econs. econs.
+      * inv RACY_WRITE.
+        exploit Thread.rtc_tau_step_non_promised; try exact STEPS0; eauto. s. i. des.
+        exploit Local.program_step_non_promised; [econs 3|..]; try exact STEP; eauto. i. des.
+        econs; eauto; try congr.
+        inv RACE. econs. rewrite TVIEW in TS.
+        inv STEP. ss.
+        apply TimeFacts.join_spec_lt; auto.
+        unfold TimeMap.singleton, Loc.LocFun.add, Loc.LocFun.init, Loc.LocFun.find. condtac; ss.
+        eapply TimeFacts.le_lt_lt; eauto. apply Time.bot_spec.
+    + ss.
 Qed.
